Libs/PartialOrder.v
@@ -1,13 +1,19 @@
-Require Export Containers.OrderedType Setoid Coq.Classes.Morphisms Computable.
-Require Import Containers.OrderedTypeEx DecSolve MoreList.
+Require Import Util LengthEq.
+Require Import Containers.OrderedType Setoid Coq.Classes.Morphisms Computable
+        Coq.Classes.RelationClasses.
+Require Import Containers.OrderedTypeEx DecSolve MoreList OrderedTypeEx.
 
 Class PartialOrder (Dom:Type) := {
   poLe : Dom -> Dom -> Prop;
   poLe_dec :> forall d d', Computable (poLe d d');
   poEq : Dom -> Dom -> Prop;
-  poEq_dec :> forall d d', Computable (poEq d d')
+  poEq_dec :> forall d d', Computable (poEq d d');
+  poEq_refl : forall d d', poEq d d' -> poLe d d';
+  poEq_equivalence :> Equivalence poEq;
+  po_antisymmetric :> Antisymmetric _ poEq poLe;
 }.
 
+Definition poLt {Dom} `{PartialOrder Dom} x y := poLe x y /\ ~ poEq x y.
 
 Instance PartialOrder_pair_instance X `{PartialOrder X} Y `{PartialOrder Y}
 : PartialOrder (X * Y) := {
@@ -16,6 +22,14 @@ Instance PartialOrder_pair_instance X `{PartialOrder X} Y `{PartialOrder Y}
   poEq x y := poEq (fst x) (fst y) /\ poEq (snd x) (snd y);
   poEq_dec := _
 }.
+Proof.
+  - intros; dcr; split; eapply poEq_refl; eauto.
+  - econstructor.
+    + hnf; intros; split; reflexivity.
+    + hnf; intros; dcr; split; symmetry; eauto.
+    + hnf; intros; dcr; split; etransitivity; eauto.
+  - intros. dcr; split; eapply po_antisymmetric; eauto.
+Defined.
 
 Instance PartialOrder_list_instance X `{PartialOrder X}
 : PartialOrder (list X) := {
@@ -24,3 +38,9 @@ Instance PartialOrder_list_instance X `{PartialOrder X}
   poEq := list_eq poEq;
   poEq_dec := _
 }.
+Proof.
+  - intros. general induction H0; eauto using @list_eq, poEq_refl.
+  - intros ? ? EQ1 EQ2.
+    exploit list_eq_length as LEN; eauto. length_equify.
+    general induction LEN; inv EQ1; inv EQ2; eauto using @list_eq, po_antisymmetric.
+Defined.
